proof-libs/coq/coq/src/Hacspec_Integers.v
@@ -55,10 +55,12 @@ Qed.
 
 (*** Hacspec Integers *)
 
-Module HacspecIntegers (WS : WORDSIZE).
+Class MyAdd (A : Type) := myadd : A -> A -> A.
+Infix ".+" := (myadd) (at level 77) : hacspec_scope.
 
+Module HacspecIntegers (WS : WORDSIZE).
+  Include (Make WS).
   (**** Public integers *)
-  Include Make WS.
 
   Definition pub (n : Z) : int := repr n.
 
@@ -78,8 +80,10 @@ Module HacspecIntegers (WS : WORDSIZE).
   Infix "shift_left" := (shift_left_) (at level 77) : hacspec_scope.
   Infix "shift_right" := (shift_right_) (at level 77) : hacspec_scope.
 
+  Instance MyAddInstance : MyAdd int := add.
+  
   Infix "%%" := Z.rem (at level 40, left associativity) : Z_scope.
-  Infix ".+" := (add) (at level 77) : hacspec_scope.
+  (* Infix ".+" := (add) (at level 77) : hacspec_scope. *)
   Infix ".-" := (sub) (at level 77) : hacspec_scope.
   Notation "-" := (neg) (at level 77) : hacspec_scope.
   Infix ".*" := (mul) (at level 77) : hacspec_scope.
@@ -93,170 +97,170 @@ Module HacspecIntegers (WS : WORDSIZE).
   (* Definition zero := (@zero WORDSIZE32). *)
   Notation "A × B" := (prod A B) (at level 79, left associativity) : hacspec_scope.
 
-(*** Uint size util *)
+  (*** Uint size util *)
 
-(* If a natural number is in bound then a smaller natural number is still in bound *)
-Lemma range_of_nat_succ :
-  forall i, (Z.pred 0 < Z.of_nat (S i) < modulus)%Z -> (Z.pred 0 < Z.of_nat i < modulus)%Z.
-Proof. lia. Qed.
+  (* If a natural number is in bound then a smaller natural number is still in bound *)
+  Lemma range_of_nat_succ :
+    forall i, (Z.pred 0 < Z.of_nat (S i) < modulus)%Z -> (Z.pred 0 < Z.of_nat i < modulus)%Z.
+  Proof. lia. Qed.
 
-(* Conversion to equivalent bound *)
-Lemma modulus_range_helper :
-  forall i, (Z.pred 0 < i < modulus)%Z -> (0 <= i <= max_unsigned)%Z.
-Proof. unfold max_unsigned. lia. Qed.
+  (* Conversion to equivalent bound *)
+  Lemma modulus_range_helper :
+    forall i, (Z.pred 0 < i < modulus)%Z -> (0 <= i <= max_unsigned)%Z.
+  Proof. unfold max_unsigned. lia. Qed.
 
-Definition unsigned_repr_alt (a : Z) `((Z.pred 0 < a < modulus)%Z) : unsigned (repr a) = a :=
-  unsigned_repr a (modulus_range_helper a H).
+  Definition unsigned_repr_alt (a : Z) `((Z.pred 0 < a < modulus)%Z) : unsigned (repr a) = a :=
+    unsigned_repr a (modulus_range_helper a H).
 
-Theorem zero_always_modulus  : (Z.pred 0 < 0 < modulus)%Z.
-Proof. easy. Qed.
+  Theorem zero_always_modulus  : (Z.pred 0 < 0 < modulus)%Z.
+  Proof. easy. Qed.
 
-(* any uint_size can be .represented as a natural number and a bound *)
-(* this is easier for proofs, however less efficient for computation *)
-(* as Z uses a binary .representation *)
-Theorem int_as_nat :
-  forall (us: int),
-    { n : nat |
-      us = repr (Z.of_nat n) /\ (Z.pred 0 < Z.of_nat n < modulus)%Z}.
-Proof.
-  destruct us as [intval intrange].
-  exists (Z.to_nat intval).
-  rewrite Z2Nat.id by (apply Z.lt_pred_le ; apply intrange).
+  (* any uint_size can be .represented as a natural number and a bound *)
+  (* this is easier for proofs, however less efficient for computation *)
+  (* as Z uses a binary .representation *)
+  Theorem int_as_nat :
+    forall (us: int),
+      { n : nat |
+        us = repr (Z.of_nat n) /\ (Z.pred 0 < Z.of_nat n < modulus)%Z}.
+  Proof.
+    destruct us as [intval intrange].
+    exists (Z.to_nat intval).
+    rewrite Z2Nat.id by (apply Z.lt_pred_le ; apply intrange).
 
-  split.
-  - apply mkint_eq.
-    rewrite Z_mod_modulus_eq.
-    rewrite Z.mod_small.
-    + reflexivity.
-    + lia.
-  - apply intrange.
-Qed.
+    split.
+    - apply mkint_eq.
+      rewrite Z_mod_modulus_eq.
+      rewrite Z.mod_small.
+      + reflexivity.
+      + lia.
+    - apply intrange.
+  Qed.
 
-(* destruct int as you would a natural number *)
-Definition destruct_int_as_nat  (a : int) : forall (P : int -> Prop),
+  (* destruct int as you would a natural number *)
+  Definition destruct_int_as_nat  (a : int) : forall (P : int -> Prop),
     forall (zero_case : P (repr 0)),
     forall (succ_case : forall (n : nat), (Z.pred 0 < Z.of_nat n < modulus)%Z -> P (repr (Z.of_nat n))),
-    P a.
-Proof.
-  intros.
-  destruct (int_as_nat a) as [ n y ] ; destruct y as [ya yb] ; subst.
-  destruct n.
-  - apply zero_case.
-  - apply succ_case.
-    apply yb.
-Qed.
-
-Ltac destruct_int_as_nat a :=
-  generalize dependent a ;
-  intros a ;
-  apply (destruct_int_as_nat a) ; [ pose proof (@unsigned_repr_alt 0 zero_always_modulus) | let n := fresh in let H := fresh in intros n H ; pose proof (@unsigned_repr_alt _ H)] ; intros.
-
-(* induction for int as you would do for a natural number *)
-Definition induction_int_as_nat :
-  forall (P : int -> Prop),
-    (P (repr 0)) ->
-    (forall n,
-        (Z.pred 0 < Z.succ (Z.of_nat n) < @modulus)%Z ->
-        P (repr (Z.of_nat n)) ->
-        P (repr (Z.succ (Z.of_nat n)))) ->
-    forall (a : int), P a.
-Proof.
-  intros P H_zero H_ind a.
-  destruct (int_as_nat a) as [ n y ] ; destruct y as [ya yb] ; subst.
-  induction n.
-  - apply H_zero.
-  - rewrite Nat2Z.inj_succ.
-    apply H_ind.
-    + rewrite <- Nat2Z.inj_succ.
+      P a.
+  Proof.
+    intros.
+    destruct (int_as_nat a) as [ n y ] ; destruct y as [ya yb] ; subst.
+    destruct n.
+    - apply zero_case.
+    - apply succ_case.
       apply yb.
-    + apply IHn.
-      lia.
-Qed.
+  Qed.
 
-Ltac induction_int_as_nat var :=
-  generalize dependent var ;
-  intros var ;
-  apply induction_int_as_nat with (a := var) ; [ pose proof (@unsigned_repr_alt 0 zero_always_modulus) | let n := fresh in let IH := fresh in intros n IH ; pose proof (@unsigned_repr_alt _ IH)] ; intros.
+  Ltac destruct_int_as_nat a :=
+    generalize dependent a ;
+    intros a ;
+    apply (destruct_int_as_nat a) ; [ pose proof (@unsigned_repr_alt 0 zero_always_modulus) | let n := fresh in let H := fresh in intros n H ; pose proof (@unsigned_repr_alt _ H)] ; intros.
 
-(* conversion of usize to positive or zero and the respective bound *)
-Theorem int_as_positive :
-  forall (us: int),
-    { pu : unit + positive |
-      match pu with inl u => us = repr Z0 | inr p => us = repr (Z.pos p) /\ (Z.pred 0 < Z.pos p < @modulus)%Z end
+  (* induction for int as you would do for a natural number *)
+  Definition induction_int_as_nat :
+    forall (P : int -> Prop),
+      (P (repr 0)) ->
+      (forall n,
+          (Z.pred 0 < Z.succ (Z.of_nat n) < @modulus)%Z ->
+          P (repr (Z.of_nat n)) ->
+          P (repr (Z.succ (Z.of_nat n)))) ->
+      forall (a : int), P a.
+  Proof.
+    intros P H_zero H_ind a.
+    destruct (int_as_nat a) as [ n y ] ; destruct y as [ya yb] ; subst.
+    induction n.
+    - apply H_zero.
+    - rewrite Nat2Z.inj_succ.
+      apply H_ind.
+      + rewrite <- Nat2Z.inj_succ.
+        apply yb.
+      + apply IHn.
+        lia.
+  Qed.
+
+  Ltac induction_int_as_nat var :=
+    generalize dependent var ;
+    intros var ;
+    apply induction_int_as_nat with (a := var) ; [ pose proof (@unsigned_repr_alt 0 zero_always_modulus) | let n := fresh in let IH := fresh in intros n IH ; pose proof (@unsigned_repr_alt _ IH)] ; intros.
+
+  (* conversion of usize to positive or zero and the respective bound *)
+  Theorem int_as_positive :
+    forall (us: int),
+      { pu : unit + positive |
+        match pu with inl u => us = repr Z0 | inr p => us = repr (Z.pos p) /\ (Z.pred 0 < Z.pos p < @modulus)%Z end
       }.
-Proof.
-  destruct us as [intval intrange].
-  destruct intval.
-  - exists (inl tt). apply mkint_eq. reflexivity.
-  - exists (inr p).
-    split.
-    + apply mkint_eq.
-      rewrite Z_mod_modulus_eq.
-      symmetry.
-      apply Zmod_small.
+  Proof.
+    destruct us as [intval intrange].
+    destruct intval.
+    - exists (inl tt). apply mkint_eq. reflexivity.
+    - exists (inr p).
+      split.
+      + apply mkint_eq.
+        rewrite Z_mod_modulus_eq.
+        symmetry.
+        apply Zmod_small.
+        lia.
+      + apply intrange.
+    - exfalso.
       lia.
-    + apply intrange.
-  - exfalso.
-    lia.
-Defined.
+  Defined.
 
-(* destruction of int as positive *)
-Definition destruct_int_as_positive  (a : int) : forall (P : int -> Prop),
-    (P (repr 0)) ->
-    (forall b, (Z.pred 0 < Z.pos b < @modulus)%Z -> P (repr (Z.pos b))) ->
-    P a.
-Proof.
-  intros P H_zero H_succ.
-  destruct (int_as_positive a) as [ [ _ | b ] y ] ; [ subst | destruct y as [ya yb] ; subst ].
-  - apply H_zero.
-  - apply H_succ.
-    apply yb.
-Qed.
+  (* destruction of int as positive *)
+  Definition destruct_int_as_positive  (a : int) : forall (P : int -> Prop),
+      (P (repr 0)) ->
+      (forall b, (Z.pred 0 < Z.pos b < @modulus)%Z -> P (repr (Z.pos b))) ->
+      P a.
+  Proof.
+    intros P H_zero H_succ.
+    destruct (int_as_positive a) as [ [ _ | b ] y ] ; [ subst | destruct y as [ya yb] ; subst ].
+    - apply H_zero.
+    - apply H_succ.
+      apply yb.
+  Qed.
 
-Ltac destruct_int_as_positive a :=
-  generalize dependent a ;
-  intros a ;
-  apply (destruct_int_as_positive a) ; intros.
+  Ltac destruct_int_as_positive a :=
+    generalize dependent a ;
+    intros a ;
+    apply (destruct_int_as_positive a) ; intros.
 
-(* induction of int as positive *)
-Definition induction_int_as_positive :
-  forall (P : int -> Prop),
-    (P (repr 0)) ->
-    (P (repr 1)) ->
-    (forall b,
-        (Z.pred 0 < Z.succ (Z.pos b) < @modulus)%Z ->
-        P (repr (Z.pos b)) ->
-        P (repr (Z.succ (Z.pos b)))) ->
-    forall (a : int), P a.
-Proof.
-  intros P H_zero H_one H_ind a.
+  (* induction of int as positive *)
+  Definition induction_int_as_positive :
+    forall (P : int -> Prop),
+      (P (repr 0)) ->
+      (P (repr 1)) ->
+      (forall b,
+          (Z.pred 0 < Z.succ (Z.pos b) < @modulus)%Z ->
+          P (repr (Z.pos b)) ->
+          P (repr (Z.succ (Z.pos b)))) ->
+      forall (a : int), P a.
+  Proof.
+    intros P H_zero H_one H_ind a.
 
-  destruct (int_as_positive a) as [ [ _ | b ] y ] ; [ subst | destruct y as [ya yb] ; subst ].
-  - apply H_zero.
-  - pose proof (pos_succ_b := positive_to_positive_succs b)
-    ; symmetry in pos_succ_b
-    ; rewrite pos_succ_b in *
-    ; clear pos_succ_b.
+    destruct (int_as_positive a) as [ [ _ | b ] y ] ; [ subst | destruct y as [ya yb] ; subst ].
+    - apply H_zero.
+    - pose proof (pos_succ_b := positive_to_positive_succs b)
+      ; symmetry in pos_succ_b
+      ; rewrite pos_succ_b in *
+      ; clear pos_succ_b.
 
-    generalize dependent (Nat.neq_sym 0 (Pos.to_nat b) (Nat.lt_neq 0 (Pos.to_nat b) (Pos2Nat.is_pos b))).
+      generalize dependent (Nat.neq_sym 0 (Pos.to_nat b) (Nat.lt_neq 0 (Pos.to_nat b) (Pos2Nat.is_pos b))).
 
-    induction (Pos.to_nat b).
-    + contradiction.
-    + intros n_neq yb.
-      destruct n.
-      * apply H_one.
-      * rewrite (positive_is_succs _  (Nat.neq_succ_0 n) n_neq) in *.
-        rewrite Pos2Z.inj_succ in *.
-        apply H_ind.
-        -- apply yb.
-        -- apply IHn.
-           lia.
-Qed.
+      induction (Pos.to_nat b).
+      + contradiction.
+      + intros n_neq yb.
+        destruct n.
+        * apply H_one.
+        * rewrite (positive_is_succs _  (Nat.neq_succ_0 n) n_neq) in *.
+          rewrite Pos2Z.inj_succ in *.
+          apply H_ind.
+          -- apply yb.
+          -- apply IHn.
+             lia.
+  Qed.
 
-Ltac induction_int_as_positive var :=
-  generalize dependent var ;
-  intros var ;
-  apply induction_int_as_positive with (a := var) ; intros ; [ | | ].
+  Ltac induction_int_as_positive var :=
+    generalize dependent var ;
+    intros var ;
+    apply induction_int_as_positive with (a := var) ; intros ; [ | | ].
 
 End HacspecIntegers.
 
@@ -276,11 +280,23 @@ Module Int32 := HacspecIntegers Wordsize_32.
 Module Int64 := HacspecIntegers Wordsize_64.
 Module Int128 := HacspecIntegers Wordsize_128.
 
+Import Int128. Export Int128.
+Import Int64. Export Int64.
+Import Int32. Export Int32.
+Import Int16. Export Int16.
+Import Int8. Export Int8.
+
 Definition int8 := Int8.int.
 Definition int16 := Int16.int.
 Definition int32 := Int32.int.
 Definition int64 := Int64.int.
 Definition int128 := Int128.int.
+
+(* Instance int8_add : MyAdd int8 := Int8.add. *)
+(* Instance int16_add : MyAdd int16 := Int16.add. *)
+(* Instance int32_add : MyAdd int32 := Int32.add. *)
+(* Instance int64_add : MyAdd int64 := Int64.add. *)
+(* Instance int128_add : MyAdd int128 := Int128.add. *)
 
 (* CompCert integers' signedness is only interpreted through 'signed' and 'unsigned',
    and not in the representation. Therefore, uints are just names for their respective ints.
@@ -343,3 +359,5 @@ Global Instance Z_Int_sizable : Int_sizable Z := {
   isize n := Int32.repr n;
   from_int_size n := Int32.signed n;
 }.
+
+Notation secret := id.
