proof-libs/coq/coq/src/Hacspec_TODO.v
@@ -1,0 +1,21 @@
+Global Set Warnings "-ambiguous-paths".
+Global Set Warnings "-uniform-inheritance".
+Global Set Warnings "-auto-template".
+Global Set Warnings "-disj-pattern-notation".
+
+From Coq Require Import ZArith List.
+Import ListNotations.
+(* Require Import IntTypes. *)
+
+(* Require Import MachineIntegers. *) From compcert Require Import Integers.
+From Coqprime Require GZnZ.
+
+Require Import Lia.
+
+(*** TODO *)
+
+Declare Scope hacspec_scope.
+Definition never_to_any {A} (f : False) : A. contradiction. Defined.
+Definition panic_fmt {A} (x : A): False. Admitted.
+Notation impl_2__new_const := id.
+Notation unsize := id.
